MonadTrans.v
@@ -1,0 +1,48 @@
+Require Coq.Lists.List.
+Require Export TypeClassLib.Monad.
+
+
+(** Example. *)
+Definition optionT (M : Type -> Type) (A : Type) := M (option A).
+
+Module OptionTFunctorSpec (MS : MonadSpec) <: FunctorSpec.
+  Definition M := MS.M.
+
+  Definition F : Type -> Type := optionT M.
+
+  Definition fmap {A B : Type} (f : A -> B) (m : optionT M A) : optionT M B :=
+    MS.fmap (OptionFunctorSpec.fmap f) m.
+
+  Lemma fmap_id : forall {A : Type},
+      fmap (fun x : A => x) = (fun x : optionT M A => x).
+  Proof.
+    intros. unfold fmap.
+    rewrite OptionFunctorSpec.fmap_id.
+    apply MS.fmap_id.
+  Qed.
+
+  Lemma fmap_compose : forall {A B C : Type} (f : A -> B) (g : B -> C),
+      fmap (g ∘ f) = fmap g ∘ fmap f.
+  Proof.
+    intros. unfold fmap.
+    rewrite OptionFunctorSpec.fmap_compose.
+    rewrite MS.fmap_compose. reflexivity.
+  Qed.
+End OptionTFunctorSpec.
+
+
+(* Instance OptionTFunctor (M : Type -> Type) `{Monad M} : Functor (optionT M) :=
+  { fmap _ _ := ; }. *)
+
+(** * The Monad Transformer Type Class *)
+
+(* TODO: Confusing to properly generalize...
+Class MonadTrans
+      (T : (Type -> Type) -> Type -> Type)
+      (M : Type -> Type) `{Monad M} :=
+  { lift : forall {A : Type}, M A -> T M A;
+    MonadTrans_Monad :> Monad (T M);
+  }.
+    lift_bind : forall {A B : Type} (m : M A) (f : A -> M B),
+        lift (bind m f) = bind (lift m) (lift ∘ f);
+  }. *)
