Makefile
@@ -7,7 +7,7 @@ all: Makefile.coq
 	+make -f Makefile.coq all
 
 clean: Makefile.coq
-	+make -f Makefile.coq clean
+	+make -f Makefile.coq cleanall
 	rm -f Makefile.coq
 
 Makefile.coq: _CoqProject Makefile
